Add Advanced Encryption Standard New Instructions (AES-NI)

x86/proofs/aes.ml
@@ -1,0 +1,33 @@
+(*
+ * Copyright Amazon.com, Inc. or its affiliates. All Rights Reserved.
+ * SPDX-License-Identifier: Apache-2.0 OR ISC OR MIT-0
+ *)
+
+(* References:
+   Intel 64 and IA-32 Architectures Software Developer's Manual Volume 1:
+     Basic Architecture, page 311-316
+   Intel 64 and IA-32 Architectures Software Developer's Manual Volume 2:
+     Instruction Set Reference, A-Z, 2A 3-63
+   White Paper: Intel Advanced Encryption Standard (AES) New Instructions Set *)
+
+let aesenc = new_definition
+ `aesenc (state:(128)word) (roundkey:(128)word) : (128)word =
+   let state = aes_shift_rows state in
+   let state = aes_sub_bytes joined_GF2 state in
+   let state = aes_mix_columns state in
+   (word_xor state roundkey)`;;
+
+let AESENC_HELPER_CONV =
+  REWRITE_CONV [aesenc] THENC
+  AES_SHIFT_ROWS_CONV THENC
+  AES_SUB_BYTES_CONV THENC
+  AES_MIX_COLUMNS_CONV THENC
+  DEPTH_CONV (WORD_RED_CONV ORELSEC NUM_RED_CONV);;
+
+let AESENC_REDUCE_CONV tm =
+  match tm with
+    Comb(Comb(Const("aesenc",_),
+         Comb(Const("word",_),state)),
+         Comb(Const("word",_),roundkey))
+    when is_numeral state && is_numeral roundkey -> AESENC_HELPER_CONV tm
+    | _ -> failwith "AESENC_REDUCE_CONV: inapplicable";;
